Common/Traces.v
@@ -1,0 +1,40 @@
+Require Import Lib.Extra.
+Require Import CompCert.Events.
+Require Import Common.Definitions.
+Require Import Common.Linking.
+
+Inductive stack_state := StackState {
+  (* The current running component.  *)
+  cur_comp : Component.id;
+
+  (* Other running components further down the stack. *)
+  callers  : list Component.id
+}.
+
+Fixpoint well_bracketed_trace (s: stack_state) (t: trace) : Prop :=
+  match t with
+  | [] => True
+  | e :: t' =>
+    cur_comp s = cur_comp_of_event e /\
+    match e with
+    | ECall C _ _ C' =>
+      well_bracketed_trace (StackState C' (C :: callers s)) t'
+    | ERet C _ C' =>
+      match callers s with
+      | [] => False
+      | head :: tail =>
+        head = C' /\
+        well_bracketed_trace (StackState C' tail) t'
+      end
+    end
+  end.
+
+Definition well_formed_event intf (e: event) : Prop :=
+  match e with
+  | ECall C P _ C' => C <> C' /\ imported_procedure intf C C' P
+  | ERet  C _   C' => C <> C'
+  end.
+
+Definition well_formed_trace intf (t: trace) : Prop :=
+  well_bracketed_trace (StackState Component.main []) t /\
+  All (well_formed_event intf) t.
